initializers: Readability
Also,

- Simplify the statement of `default_initialize_array_frame`

theories/lang/cpp/logic/initializers.v
@@ -1,5 +1,5 @@
 (*
- * Copyright (c) 2020 BedRock Systems, Inc.
+ * Copyright (c) 2020-2023 BedRock Systems, Inc.
  * This software is distributed under the terms of the BedRock Open-Source License.
  * See the LICENSE-BedRock file in the repository root for details.
  *)
@@ -12,263 +12,288 @@ Require Import bedrock.lang.bi.errors.
 From bedrock.lang.cpp.logic Require Import
      pred path_pred heap_pred wp destroy const.
 
-(** The C++ language provides several types of initialization:
-    - default initialization <https://eel.is/c++draft/dcl.init#def:default-initialization>
-    - value initialization <https://eel.is/c++draft/dcl.init#def:value-initialization>
-    - zero initialization <https://eel.is/c++draft/dcl.init#def:zero-initialization>
-    - direct initialization <https://eel.is/c++draft/dcl.init#def:direct-initialization>
+(**
+The C++ language provides several types of initialization:
+- default initialization <https://eel.is/c++draft/dcl.init#def:default-initialization>
+- value initialization <https://eel.is/c++draft/dcl.init#def:value-initialization>
+- zero initialization <https://eel.is/c++draft/dcl.init#def:zero-initialization>
+- direct initialization <https://eel.is/c++draft/dcl.init#def:direct-initialization>
 
-    The BRiCk frontend resolves (via clang) the rules for which one of these is used in each
-    context. Therefore, in the semantics, we are left with only two cases:
-    - default initialization (implemented by [default_initialize]), which occurs when there
-      is no expression used to initialize the value
-    - expression initialization (implemented by [wp_initialize]), which occurs when there is
-      an expression used to initialize the value.
+The BRiCk frontend resolves (via clang) the rules for which one of
+these is used in each context. Therefore, in the semantics, we are
+left with only two cases:
 
-    Note that the frontend inserts constructor calls to default initialize objects, so
-    [Tnamed] types can *not* be default initialized.
- *)
+- default initialization (implemented by [default_initialize]), which
+occurs when there is no expression used to initialize the value
 
-Module Type Init.
+- expression initialization (implemented by [wp_initialize]), which
+occurs when there is an expression used to initialize the value.
 
-  Section with_resolve.
-    Context `{Σ : cpp_logic thread_info} {σ:genv} (tu : translation_unit).
-    Variables (ρ : region).
+Note that the frontend inserts constructor calls to default initialize
+objects, so [Tnamed] types can *not* be default initialized.
+*)
 
-    #[local] Notation wp := (wp tu ρ).
-    #[local] Notation wp_lval := (wp_lval tu ρ).
-    #[local] Notation wp_operand := (wp_operand tu ρ).
-    #[local] Notation wp_xval := (wp_xval tu ρ).
-    #[local] Notation wp_init := (wp_init tu ρ).
-    #[local] Notation interp := (interp tu).
-    #[local] Notation wp_fptr := (@wp_fptr _ Σ tu.(types)).
-    #[local] Notation mspec := (@mspec _ Σ tu.(types)).
+Section with_resolve.
+  Context `{Σ : cpp_logic thread_info} {σ:genv} (tu : translation_unit).
+  Implicit Types (Q : FreeTemps -> epred).
+  Variables (ρ : region).
 
-    (** [default_initialize_array default_init ty len p Q] initializes an array of type [ty[len]]
-        at pointer [p].
+  #[local] Notation wp := (wp tu ρ).
+  #[local] Notation wp_lval := (wp_lval tu ρ).
+  #[local] Notation wp_operand := (wp_operand tu ρ).
+  #[local] Notation wp_xval := (wp_xval tu ρ).
+  #[local] Notation wp_init := (wp_init tu ρ).
+  #[local] Notation interp := (interp tu).
+  #[local] Notation wp_fptr := (@wp_fptr _ Σ tu.(types)).
+  #[local] Notation mspec := (@mspec _ Σ tu.(types)).
 
-        NOTE that default initialization of an array of constants is a compile-time error, so
-             we don't need to worry about that case. Also, note that arrays of length 0 are
-             not legal so we are guaranteed to have to initialize a value which will result in
-             an [ERROR].
-     *)
-    Definition default_initialize_array (default_initialize : type -> ptr -> (FreeTemps -> epred) -> mpred)
-               (ty : type) (len : N) (p : ptr) (Q : FreeTemps -> epred) : mpred :=
-      fold_right (fun i PP => default_initialize ty (p ,, o_sub _ ty (Z.of_N i)) (fun free' => interp free' PP))
-                 (p .[ ty ! Z.of_N len ] |-> validR -* Q FreeTemps.id) (seqN 0 len).
-    #[global] Arguments default_initialize_array : simpl never.
+  (**
+  [default_initialize_array default_init ty len p Q] initializes an
+  array of type [ty[len]] at pointer [p].
 
-    Lemma default_initialize_array_frame : ∀ di ty sz Q Q' (p : ptr),
-        (Forall f, Q f -* Q' f)
-    |-- <pers> (Forall p Q Q', (Forall f, Q f -* Q' f) -* di ty p Q -* di ty p Q')
-          -* default_initialize_array di ty sz p Q -* default_initialize_array di ty sz p Q'.
-    Proof.
-      intros ? ? sz Q Q' p; rewrite /default_initialize_array.
-      generalize dependent (p .[ ty ! Z.of_N sz ] |-> validR).
-      induction (seqN 0 sz) =>/=; intros.
-      - iIntros "X #Y a b"; iApply "X"; iApply "a"; eauto.
-      - iIntros "F #Hty". iApply "Hty".
-        iIntros (?). iApply interp_frame. iApply (IHl with "F"); eauto.
-    Qed.
+  NOTE that default initialization of an array of constants is a
+  compile-time error, so we don't need to worry about that case.
+  Also, note that arrays of length 0 are not legal so we are
+  guaranteed to have to initialize a value which will result in an
+  [ERROR].
+  *)
+  Definition default_initialize_array
+      (default_initialize : type -> ptr -> (FreeTemps -> epred) -> mpred)
+      (ty : type) (len : N) (p : ptr) (Q : FreeTemps -> epred) : mpred :=
+    let folder i PP :=
+      default_initialize ty (p ,, o_sub _ ty (Z.of_N i)) (fun free' => interp free' PP)
+    in
+    foldr folder (p .[ ty ! Z.of_N len ] |-> validR -* Q FreeTemps.id) (seqN 0 len).
+  #[global] Arguments default_initialize_array : simpl never.
 
-    (** [default_initialize ty p Q] default initializes the memory at [p] according to
-        the type [ty].
+  Lemma default_initialize_array_frame di ty sz Q Q' (p : ptr) :
+    (∀ p Q Q', (Forall f, Q f -* Q' f) |-- di ty p Q -* di ty p Q') ->
+    (Forall f, Q f -* Q' f)
+    |-- default_initialize_array di ty sz p Q -* default_initialize_array di ty sz p Q'.
+  Proof.
+    intros IHty.
+    rewrite /default_initialize_array.
+    generalize dependent (p .[ ty ! Z.of_N sz ] |-> validR).
+    induction (seqN 0 sz) =>/=; intros.
+    - iIntros "X a b". iApply "X". by iApply "a".
+    - iIntros "F". iApply IHty.
+      iIntros (?). iApply interp_frame. iApply (IHl with "F").
+  Qed.
 
-        NOTE this assumes that the underlying memory has already been given to the
-             C++ abstract machine.
+  (**
+  [default_initialize ty p Q] default initializes the memory at [p]
+  according to the type [ty].
 
-        NOTE: <https://eel.is/c++draft/dcl.init#general-7>:
-        | (7) To default-initialize an object of type T means:
-        | (7.1) If T is a (possibly cv-qualified) class type ([class]), constructors are considered.
-        |       The applicable constructors are enumerated ([over.match.ctor]), and the best one for
-        |       the initializer () is chosen through overload resolution ([over.match]).
-        |       The constructor thus selected is called, with an empty argument list, to initialize
-        |       the object.
-        | (7.2) If T is an array type, each element is default-initialized.
-        | (7.3) Otherwise, no initialization is performed.
-        and [default_initialize] corresponds to [default-initialization] as described above.
-     *)
-    Fixpoint default_initialize (ty : type) (p : ptr) (Q : FreeTemps → epred) {struct ty} : mpred :=
-      match ty with
-      | Tnum _ _
-      | Tchar_ _
-      | Tptr _
-      | Tbool
-      | Tfloat_ _
-      | Tnullptr
-      | Tenum _ =>
-          let rty := erase_qualifiers ty in
-          p |-> uninitR rty (cQp.m 1) -* Q FreeTemps.id
+  NOTE this assumes that the underlying memory has already been
+  given to the C++ abstract machine.
 
-      | Tarray ety sz =>
-          default_initialize_array default_initialize ety sz p (fun _ => Q FreeTemps.id)
+  NOTE: <https://eel.is/c++draft/dcl.init#general-7>:
+  | (7) To default-initialize an object of type T means:
+  | (7.1) If T is a (possibly cv-qualified) class type ([class]), constructors are considered.
+  |       The applicable constructors are enumerated ([over.match.ctor]), and the best one for
+  |       the initializer () is chosen through overload resolution ([over.match]).
+  |       The constructor thus selected is called, with an empty argument list, to initialize
+  |       the object.
+  | (7.2) If T is an array type, each element is default-initialized.
+  | (7.3) Otherwise, no initialization is performed.
 
-      | Tref _
-      | Trv_ref _ => ERROR "default initialization of reference"
-      | Tvoid => ERROR "default initialization of void"
-      | Tfunction _ _ => ERROR "default initialization of functions"
-      | Tmember_pointer _ _ => ERROR "default initialization of member pointers"
-      | Tnamed _ => False (* default initialization of aggregates is done at elaboration time. *)
+  and [default_initialize] corresponds to [default-initialization]
+  as described above.
+  *)
+  Fixpoint default_initialize (ty : type) (p : ptr) (Q : FreeTemps → epred) {struct ty} : mpred :=
+    match ty with
+    | Tnum _ _
+    | Tchar_ _
+    | Tptr _
+    | Tbool
+    | Tfloat_ _
+    | Tnullptr
+    | Tenum _ =>
+      let rty := erase_qualifiers ty in
+      p |-> uninitR rty (cQp.m 1) -* Q FreeTemps.id
 
-      | Tarch _ _ => UNSUPPORTED "default initialization of architecture type"
-      | Tqualified q ty =>
-          if q_const q then ERROR "default initialize const"
-          else default_initialize ty p Q
-      end%bs%I.
-    #[global] Arguments default_initialize !_ _ _ / : assert.
+    | Tarray ety sz =>
+      default_initialize_array default_initialize ety sz p (fun _ => Q FreeTemps.id)
 
-    (** TODO this should be generalized to different [σ] but, in that case it relies
-        on the fact that [ty] is defined in both environments.
-     *)
-    Lemma default_initialize_frame ty : forall this Q Q',
-        (Forall f, Q f -* Q' f)
-        |-- default_initialize ty this Q -* default_initialize ty this Q'.
-    Proof.
-      induction ty; simpl; intros; try case_match;
-        try solve [ intros; iIntros "a b c"; iApply "a"; iApply "b"; eauto | eauto ].
-      { intros. iIntros "a"; iApply (default_initialize_array_frame with "a").
-        iModIntro. iIntros (???) "a". by iApply IHty. }
-    Qed.
+    | Tref _
+    | Trv_ref _ => ERROR "default initialization of reference"
+    | Tvoid => ERROR "default initialization of void"
+    | Tfunction _ _ => ERROR "default initialization of functions"
+    | Tmember_pointer _ _ => ERROR "default initialization of member pointers"
+    | Tnamed _ => False (* default initialization of aggregates is done at elaboration time. *)
 
-    (* error used when using [e] to initialize a value of type [ty]. *)
-    Variant initializing_type (ty : type) (e : Expr) : Prop := ANY.
+    | Tarch _ _ => UNSUPPORTED "default initialization of architecture type"
+    | Tqualified q ty =>
+      if q_const q then ERROR "default initialize const"
+      else default_initialize ty p Q
+    end%bs%I.
+  #[global] Arguments default_initialize !_ _ _ / : assert.
 
-    (** [wp_initialize] provides "constructor" semantics for types.
-        For aggregates, simply delegates to [wp_init], but for primitives,
-        the semantics is to evaluate the primitive and initialize the location
-        with the value.
+  (**
+  TODO this should be generalized to different [σ] but, in that case
+  it relies on the fact that [ty] is defined in both environments.
+  *)
+  Lemma default_initialize_frame ty : forall this Q Q',
+    (Forall f, Q f -* Q' f)
+    |-- default_initialize ty this Q -* default_initialize ty this Q'.
+  Proof.
+    induction ty; simpl; intros; try case_match;
+      try solve [ intros; iIntros "a b c"; iApply "a"; iApply "b"; eauto | eauto ].
+    { intros. iIntros "a". by iApply (default_initialize_array_frame with "a"). }
+  Qed.
 
-        NOTE this assumes that the memory is coming from the C++ abstract machine.
+  (* error used when using [e] to initialize a value of type [ty]. *)
+  Variant initializing_type (ty : type) (e : Expr) : Prop := ANY.
 
-        NOTE [wp_initialize] is very similar to [wp_init] except that [wp_initialize]
-        can be used to initialize all values (including references) whereas [wp_init]
-        is only safe to initialize non-primitives (arrays and aggregates).
-     *)
-    Definition wp_initialize (qty : type) (addr : ptr) (init : Expr) (k : FreeTemps -> mpred) : mpred :=
-      let '(cv, ty) := decompose_type qty in
-      (**
-      TODO (Gregory): In a few cases below, we're using [cQp.m 1]
-      rather than [qf]. Please add a comment explaining.
+  (**
+  [wp_initialize] provides "constructor" semantics for types. For
+  aggregates, simply delegates to [wp_init], but for primitives, the
+  semantics is to evaluate the primitive and initialize the location
+  with the value.
+
+  NOTE this assumes that the memory is coming from the C++ abstract
+  machine.
+
+  NOTE [wp_initialize] is very similar to [wp_init] except that
+  [wp_initialize] can be used to initialize all values (including
+  references) whereas [wp_init] is only safe to initialize
+  non-primitives (arrays and aggregates).
+  *)
+  Definition wp_initialize (qty : type) (addr : ptr) (init : Expr) (Q : FreeTemps -> mpred) : mpred :=
+    let '(cv, ty) := decompose_type qty in
+    (**
+    TODO (Gregory): In a few cases below, we're using [cQp.m 1]
+    rather than [qf]. Please add a comment explaining.
+    *)
+    let qf := if q_const cv then cQp.const 1 else cQp.mut 1 in
+    match ty with
+    | Tvoid =>
+      (*
+      [wp_initialize] is used to `return` from a function. The
+      following is legal in C++:
+      <<
+         void f();
+         void g() { return f(); }
+      >>
       *)
-      let qf := if q_const cv then cQp.const 1 else cQp.mut 1 in
-      match ty with
-      | Tvoid =>
-        (* [wp_initialize] is used to `return` from a function.
-           The following is legal in C++:
-           ```
-           void f();
-           void g() { return f(); }
-           ```
-         *)
-        wp_operand init (fun v frees => [| v = Vvoid |] ** (addr |-> primR Tvoid qf Vvoid -* k frees))
-      | Tpointer _ as ty
-      | Tmember_pointer _ _ as ty
-      | Tbool as ty
-      | Tnum _ _ as ty
-      | Tchar_ _ as ty
-      | Tenum _ as ty
-      | Tfloat_ _ as ty
-      | Tnullptr as ty =>
-        wp_operand init (fun v free =>
-                          addr |-> primR (erase_qualifiers ty) qf v -* k free)
+      letI* v, frees := wp_operand init in
+      [| v = Vvoid |] **
+      (addr |-> primR Tvoid qf Vvoid -* Q frees)
 
-        (* non-primitives are handled via prvalue-initialization semantics *)
-      | Tarray _ _ as ty
-      | Tnamed _ as ty => wp_init ty addr init (fun _ frees =>
-           if q_const cv then wp_make_const tu addr ty (k frees)
-           else k frees)
+    | Tpointer _
+    | Tmember_pointer _ _
+    | Tbool
+    | Tnum _ _
+    | Tchar_ _
+    | Tenum _
+    | Tfloat_ _
+    | Tnullptr =>
+      letI* v, free := wp_operand init in
+      addr |-> primR (erase_qualifiers ty) qf v -* Q free
 
-      | Tref ty =>
-        let rty := Tref $ erase_qualifiers ty in
-        wp_lval init (fun p free =>
-                        addr |-> primR rty qf (Vref p) -* k free)
-        (* ^ TODO: [ref]s are never mutable, but we use [qf] here
-           for compatibility with [implicit_destruct_struct] *)
+      (* non-primitives are handled via prvalue-initialization semantics *)
+    | Tarray _ _
+    | Tnamed _ =>
+      letI* _, frees := wp_init ty addr init in
+      letI* := if q_const cv then wp_make_const tu addr ty else id in
+      Q frees
 
-      | Trv_ref ty =>
-        let rty := Tref $ erase_qualifiers ty in
-        wp_xval init (fun p free =>
-                        addr |-> primR rty qf (Vref p) -* k free)
-        (* ^ TODO: [ref]s are never mutable, but we use [qf] here
-           for compatibility with [implicit_destruct_struct] *)
-      | Tfunction _ _ => UNSUPPORTED (initializing_type ty init)
+    | Tref ty =>
+      let rty := Tref $ erase_qualifiers ty in
+      letI* p, free := wp_lval init in
+      (*
+      TODO: [ref]s are never mutable, but we use [qf] here
+      for compatibility with [implicit_destruct_struct]
+      *)
+      addr |-> primR rty qf (Vref p) -* Q free
 
-      | Tqualified _ ty => False (* unreachable *)
-      | Tarch _ _ => UNSUPPORTED (initializing_type ty init)
-      end.
-    #[global] Arguments wp_initialize !_ _ _ _ /.
+    | Trv_ref ty =>
+      let rty := Tref $ erase_qualifiers ty in
+      letI* p, free := wp_xval init in
+      (*
+      TODO: [ref]s are never mutable, but we use [qf] here
+      for compatibility with [implicit_destruct_struct]
+      *)
+      addr |-> primR rty qf (Vref p) -* Q free
 
-    (** [wpi cls this init Q] evaluates the initializer [init] from the
-        object [thisp] (of type [Tnamed cls]) and then proceeds as [Q].
+    | Tfunction _ _ => UNSUPPORTED (initializing_type ty init)
 
-        NOTE that temporaries introduced by the evaluation of [init] are cleaned
-        up before [Q] is run ([Q] does not have a [FreeTemps] argument). This is
-        because initialization is considered a full expression.
-        See [https://eel.is/c++draft/class.init#class.base.init-note-2].
-     *)
-    Definition wpi (cls : globname) (thisp : ptr) (init : Initializer) (Q : epred) : mpred :=
-        let p' := thisp ,, offset_for cls init.(init_path) in
-        wp_initialize init.(init_type) p' init.(init_init) (fun free => interp free Q).
-    #[global] Arguments wpi _ _ _ _ /.
+    | Tqualified _ ty => False (* unreachable *)
+    | Tarch _ _ => UNSUPPORTED (initializing_type ty init)
+    end.
+  #[global] Arguments wp_initialize !_ _ _ _ /.
 
-  End with_resolve.
+  (**
+  [wpi cls this init Q] evaluates the initializer [init] from the
+  object [thisp] (of type [Tnamed cls]) and then proceeds as [Q].
 
-  #[global] Hint Opaque default_initialize_array : typeclass_instances.
+  NOTE that temporaries introduced by the evaluation of [init] are
+  cleaned up before [Q] is run ([Q] does not have a [FreeTemps]
+  argument). This is because initialization is considered a full
+  expression.
 
-  Section frames.
-    Context `{Σ : cpp_logic thread_info} {σ1 σ2 :genv} (tu : translation_unit).
-    Variables (ρ : region).
-    Hypothesis MOD : genv_leq σ1 σ2.
+  See [https://eel.is/c++draft/class.init#class.base.init-note-2].
+  *)
+  Definition wpi (cls : globname) (thisp : ptr) (init : Initializer) (Q : epred) : mpred :=
+    let p' := thisp ,, offset_for cls init.(init_path) in
+    letI* free := wp_initialize init.(init_type) p' init.(init_init) in
+    letI* := interp free in
+    Q.
+  #[global] Arguments wpi _ _ _ _ /.
 
-    Lemma wp_initialize_frame obj ty e Q Q' :
-      (Forall free, Q free -* Q' free)
-      |-- wp_initialize (σ:=σ2) tu ρ ty obj e Q -* wp_initialize (σ:=σ2) tu ρ ty obj e Q'.
-    Proof using.
-      rewrite /wp_initialize.
-      iIntros "a".
-      case: (decompose_type _)=>a; case=>>; auto; try
-          by [ iApply wp_operand_frame => //; iIntros (??) "X ?"; iApply "a"; iApply "X"
-             | iIntros "H"; iExact "H"
-             | iApply wp_init_frame => //-;
-               case: (q_const _); iIntros (??); [ iApply wp_const_frame; try reflexivity | ]; iApply "a"
-             ].
-      { by iApply wp_lval_frame => //; iIntros (??) "X ?"; iApply "a"; iApply "X". }
-      { by iApply wp_xval_frame => //; iIntros (??) "X ?"; iApply "a"; iApply "X". }
-      { by iApply wp_operand_frame => //; iIntros (??) "[$ X] ?"; iApply "a"; iApply "X". }
-    Qed.
+End with_resolve.
 
-    Lemma wp_initialize_wand obj ty e Q Q' :
-      wp_initialize (σ:=σ2) tu ρ ty obj e Q
-      |-- (Forall free, Q free -* Q' free) -* wp_initialize (σ:=σ2) tu ρ ty obj e Q'.
-    Proof. by iIntros "H Y"; iRevert "H"; iApply wp_initialize_frame. Qed.
+#[global] Hint Opaque default_initialize_array : typeclass_instances.
 
-    Theorem wpi_frame (cls : globname) (this : ptr) (e : Initializer) k1 k2 :
-      k1 -* k2 |-- wpi (σ:=σ1) tu ρ cls this e k1 -* wpi (σ:=σ2) tu ρ cls this e k2.
-    Proof. Abort. (* This is not provable *)
-  End frames.
+Section frames.
+  Context `{Σ : cpp_logic thread_info} {σ1 σ2 :genv} (tu : translation_unit).
+  Variables (ρ : region).
+  Hypothesis MOD : genv_leq σ1 σ2.
 
-  Section mono_frames.
-    (* All framing lemmas *should* work with [genv] weakening, but that
-       requires some additional side-conditions on paths that we can't prove
-       right now. So, for the time being, we prove [_frame] lemmas without
-       [genv] weakening.
-     *)
+  Lemma wp_initialize_frame obj ty e Q Q' :
+    (Forall free, Q free -* Q' free)
+    |-- wp_initialize (σ:=σ2) tu ρ ty obj e Q -* wp_initialize (σ:=σ2) tu ρ ty obj e Q'.
+  Proof using.
+    rewrite /wp_initialize.
+    iIntros "a".
+    case: (decompose_type _)=>a; case=>>; auto; try
+        by [ iApply wp_operand_frame => //; iIntros (??) "X ?"; iApply "a"; iApply "X"
+           | iIntros "H"; iExact "H"
+           | iApply wp_init_frame => //-;
+             case: (q_const _); iIntros (??); [ iApply wp_const_frame; try reflexivity | ]; iApply "a"
+           ].
+    { by iApply wp_lval_frame => //; iIntros (??) "X ?"; iApply "a"; iApply "X". }
+    { by iApply wp_xval_frame => //; iIntros (??) "X ?"; iApply "a"; iApply "X". }
+    { by iApply wp_operand_frame => //; iIntros (??) "[$ X] ?"; iApply "a"; iApply "X". }
+  Qed.
 
-    Context `{Σ : cpp_logic thread_info} {σ : genv} (tu : translation_unit).
-    Variables (ρ : region).
+  Lemma wp_initialize_wand obj ty e Q Q' :
+    wp_initialize (σ:=σ2) tu ρ ty obj e Q
+    |-- (Forall free, Q free -* Q' free) -* wp_initialize (σ:=σ2) tu ρ ty obj e Q'.
+  Proof. by iIntros "H Y"; iRevert "H"; iApply wp_initialize_frame. Qed.
 
-    Theorem wpi_frame (cls : globname) (this : ptr) (e : Initializer) k1 k2 :
-      k1 -* k2 |-- wpi tu ρ cls this e k1 -* wpi tu ρ cls this e k2.
-    Proof.
-      clear.
-      iIntros "X". rewrite /wpi. iApply wp_initialize_frame.
-      iIntros (?); by iApply interp_frame.
-    Qed.
+  Theorem wpi_frame (cls : globname) (this : ptr) (e : Initializer) k1 k2 :
+    k1 -* k2 |-- wpi (σ:=σ1) tu ρ cls this e k1 -* wpi (σ:=σ2) tu ρ cls this e k2.
+  Proof. Abort. (* This is not provable *)
+End frames.
 
-  End mono_frames.
+Section mono_frames.
+  (*
+  All framing lemmas *should* work with [genv] weakening, but that
+  requires some additional side-conditions on paths that we can't
+  prove right now. So, for the time being, we prove [_frame] lemmas
+  without [genv] weakening.
+  *)
 
-End Init.
+  Context `{Σ : cpp_logic thread_info} {σ : genv} (tu : translation_unit).
+  Variables (ρ : region).
 
-Declare Module IN : Init.
+  Theorem wpi_frame (cls : globname) (this : ptr) (e : Initializer) k1 k2 :
+    k1 -* k2 |-- wpi tu ρ cls this e k1 -* wpi tu ρ cls this e k2.
+  Proof.
+    clear.
+    iIntros "X". rewrite /wpi. iApply wp_initialize_frame.
+    iIntros (?); by iApply interp_frame.
+  Qed.
 
-Export IN.
+End mono_frames.
